ReactorModel/Execution/Theorems/Execution.lean
@@ -1,4 +1,4 @@
-import ReactorModel.Execution.Theorems.Trivial 
+import ReactorModel.Execution.Theorems.Trivial
 import ReactorModel.Execution.Theorems.Grouped.Basic
 
 open Classical Reactor
@@ -7,10 +7,11 @@ namespace Execution
 
 variable [Proper α] {s : State α}
 
-theorem deterministic 
-    (e₁ : s ⇓ s₁) (e₂ : s ⇓ s₂) (ht : s₁.tag = s₂.tag) (hp : s₁.progress = s₂.progress) : s₁ = s₂ := 
-  if h : s.Nontrivial 
-  then (e₁.to_grouped h).some.deterministic h ht hp (e₂.to_grouped h).some
+theorem deterministic
+    (e₁ : Execution s s₁) (e₂ : Execution s s₂) (ht : s₁.tag = s₂.tag)
+    (hp : s₁.progress = s₂.progress) : s₁ = s₂ :=
+  if h : s.Nontrivial
+  then (e₁.to_grouped h).deterministic h ht hp (e₂.to_grouped h)
   else e₁.trivial_deterministic h e₂ ht
-  
+
 end Execution
