ReactorModel/Execution/Theorems/Monotonicity.lean
@@ -7,7 +7,7 @@ namespace Execution
 variable [Proper α] {s₁ s₂ : State α}
 
 -- Property (1) on page 10 of https://www.informatik.uni-bremen.de/agbs/jp/papers/trs_script.pdf.
-theorem tag_le (e : s₁ ⇓ s₂) : s₁.tag ≤ s₂.tag := by
+theorem tag_le (e : Execution s₁ s₂) : s₁.tag ≤ s₂.tag := by
   induction e
   case refl           => rfl
   case trans e₁ e₂ ih => exact e₁.tag_le.trans ih
