ReactorModel/Execution/Theorems/Progress.lean
@@ -14,7 +14,7 @@ namespace Progress
 theorem to_deps_acyclic [Hierarchical α] {rtr : α} (p : Progress rtr) : Dependency.Acyclic rtr := by
   simp [Dependency.Acyclic.iff_mem_acyclic]
   intro rcn hm
-  have ⟨_, e⟩ := p _ <| State.Over.forcing_not_terminal hm
+  have ⟨_, ⟨e⟩⟩ := p _ <| State.Over.forcing_not_terminal hm
   cases e
   case time e => exact State.Over.forcing_not_time_step e hm |>.elim
   case skip e => exact State.Over.forcing_skip_step_rcn_eq e ▸ e.allows_rcn.acyclic
@@ -26,12 +26,12 @@ theorem of_deps_acyclic (a : Dependency.Acyclic rtr) : Progress rtr :=
   fun s ht =>
     if hc : s.Closed then
       let ⟨_, hg⟩ := State.Terminal.not_elim ht |>.resolve_left (not_not.mpr hc)
-      ⟨_, .time ⟨hc, hg, refresh_correct _ <| Partial.mapIdx_ids ..⟩⟩
+      ⟨_, ⟨.time ⟨hc, hg, refresh_correct _ <| Partial.mapIdx_ids ..⟩⟩⟩
     else
       let ⟨rcn, hr⟩ := s.exists_allowed_of_acyclic_not_closed a hc
       if h : s.Triggers rcn
-      then ⟨_, .exec ⟨hr, h, Step.Apply.RTC.construct .. |>.snd⟩⟩
-      else ⟨_, .skip ⟨hr, h⟩⟩
+      then ⟨_, ⟨.exec ⟨hr, h, Step.Apply.RTC.construct .. |>.snd⟩⟩⟩
+      else ⟨_, ⟨.skip ⟨hr, h⟩⟩⟩
 
 theorem iff_deps_acyclic : (Progress rtr) ↔ (Dependency.Acyclic rtr) :=
   ⟨to_deps_acyclic, of_deps_acyclic⟩
