ReactorModel/Execution/Theorems/Step/Basic.lean
@@ -8,6 +8,6 @@ variable [Hierarchical α] {s₁ s₂ : State α}
 
 namespace Execution.Step
 
-theorem tag_le : (s₁ ↓ s₂) → s₁.tag ≤ s₂.tag
+theorem tag_le : (Step s₁ s₂) → s₁.tag ≤ s₂.tag
   | .skip e | .exec e => le_of_eq e.preserves_tag
   | .time e           => le_of_lt e.tag_lt
